HoareLogic: proved triple for [begin]

HoareLogic.v
@@ -1,4 +1,4 @@
-Require Import Arith.
+Require Import Arith Omega List.
 
 Set Implicit Arguments.
 
@@ -10,14 +10,15 @@ Definition valu := nat.
 
 Inductive prog :=
 | Halt
+| Crash
 | Read (a : addr)
 | Write (a : addr) (v : valu)
 | Seq (p1 : prog) (p2 : valu -> prog).
 
 Notation "!" := Read.
 Infix "<--" := Write (at level 8).
-Notation "p1 ;; p2" := (Seq p1 (fun _ => p2)) (at level 9).
-Notation "x <- p1 ; p2" := (Seq p1 (fun x => p2)) (at level 9).
+Notation "p1 ;; p2" := (Seq p1 (fun _ => p2)) (at level 9, right associativity).
+Notation "x <- p1 ; p2" := (Seq p1 (fun x => p2)) (at level 9, right associativity).
 
 Definition mem := addr -> valu.
 Definition mem0 : mem := fun _ => 0.
@@ -52,6 +53,10 @@ Infix "|->" := ptsto (at level 40) : pred_scope.
 Bind Scope pred_scope with pred.
 Delimit Scope pred_scope with pred.
 
+Definition impl (p q : pred) : pred :=
+  fun m => p m -> q m.
+Infix "-->" := impl (right associativity, at level 95) : pred_scope.
+
 Definition and (p q : pred) : pred :=
   fun m => p m /\ q m.
 Infix "/\" := and : pred_scope.
@@ -59,6 +64,10 @@ Infix "/\" := and : pred_scope.
 Definition or (p q : pred) : pred :=
   fun m => p m \/ q m.
 Infix "\/" := or : pred_scope.
+
+Definition foral_ A (p : A -> pred) : pred :=
+  fun m => forall x, p x m.
+Notation "'foral' x .. y , p" := (foral_ (fun x => .. (foral_ (fun y => p)) ..)) (at level 200, x binder, right associativity) : pred_scope.
 
 Definition exis A (p : A -> pred) : pred :=
   fun m => exists x, p x m.
@@ -69,11 +78,13 @@ Definition lift (P : Prop) : pred :=
 Notation "[ P ]" := (lift P) : pred_scope.
 
 Definition pimpl (p q : pred) := forall m, p m -> q m.
-Notation "p --> q" := (pimpl p%pred q%pred) (at level 95).
+Notation "p --> q" := (pimpl p%pred q%pred).
 
 Definition pupd (p : pred) (a : addr) (v : valu) : pred :=
   fun m => exists m', p m' /\ m = upd m' a v.
 Notation "p [ a <--- v ]" := (pupd p a v) (at level 0) : pred_scope.
+
+Definition diskIs (m : mem) : pred := eq m.
 
 (** ** Hoare triples *)
 
@@ -84,6 +95,8 @@ Inductive corr :
   -> Prop :=
 | CHalt : forall pre,
   corr pre Halt (fun r => [r = Crashed \/ r = Halted 0] /\ pre)%pred
+| CCrash : forall pre,
+  corr pre Crash (fun r => [r = Crashed] /\ pre)%pred
 | CRead : forall pre a,
   corr pre (Read a) (fun r => exists v, a |-> v /\ [r = Crashed \/ r = Halted v] /\ pre)%pred
 | CWrite : forall pre a v,
@@ -91,19 +104,27 @@ Inductive corr :
 | CSeq : forall pre p1 p2 post1 post2,
   corr pre p1 post1
   -> (forall v, corr (post1 (Halted v)) (p2 v) post2)
-  -> corr pre (Seq p1 p2) (fun r => post1 Crashed \/ post2 r)%pred
+  -> corr pre (Seq p1 p2) (fun r => ([r = Crashed] /\ post1 Crashed) \/ post2 r)%pred
 | Conseq : forall pre post p pre' post', corr pre p post
   -> (pre' --> pre)
   -> (forall r, post r --> post' r)
   -> corr pre' p post'.
+
+Hint Constructors corr.
 
 Notation "{{ pre }} p {{ r , post }}" := (corr pre p (fun r => post)%pred)
   (at level 0, p at level 9).
 
 (** ** Soundness  *)
 
-Ltac pred_unfold := unfold ptsto, and, or, exis, lift, pimpl, pupd in *.
-Ltac pred := pred_unfold; intuition eauto.
+Ltac deex := match goal with
+               | [ H : ex _ |- _ ] => destruct H; intuition subst
+             end.
+
+Ltac pred_unfold := unfold ptsto, impl, and, or, foral_, exis, lift, pimpl, pupd, diskIs in *.
+Ltac pred := pred_unfold;
+  repeat (repeat deex;
+    intuition (try congruence; try autorewrite with core in *; eauto)).
 
 Lemma could_always_crash : forall pre p post, corr pre p post
   -> forall m, pre m -> post Crashed m.
@@ -124,3 +145,241 @@ Theorem corr_sound : forall pre p post, corr pre p post
 Proof.
   induction 1; solve [ pred | inversion_clear 1; pred ].
 Qed.
+
+
+(** * Some helpful [prog] combinators *)
+
+Theorem pimpl_refl : forall p, p --> p.
+Proof.
+  pred.
+Qed.
+
+Hint Resolve pimpl_refl.
+
+Fixpoint Countdown (nocrash : nat -> pred) (crashed : pred)
+  (f : nat -> prog) (n : nat) : prog :=
+  match n with
+    | O => Halt
+    | S n' => (f n');; (Countdown nocrash crashed f n')
+  end.
+
+Notation "'Loop' i < n 'Invariant' nocrash 'OnCrash' crashed 'Begin' body 'Pool'" :=
+  (Countdown (fun i => nocrash)%pred crashed (fun i => body) n)
+  (at level 9, i at level 0, n at level 0, body at level 9).
+
+Theorem CCountdown : forall (f : nat -> prog)
+  (nocrash : nat -> pred) (crashed : pred),
+  (forall n, {{nocrash (S n)}} (f n)
+    {{r, ([r = Halted 0] /\ nocrash n) \/ ([r = Crashed] /\ crashed)}})
+  -> (nocrash 0 --> crashed)
+  -> forall n, {{nocrash n}} (Countdown nocrash crashed f n)
+    {{r, ([r = Halted 0] /\ nocrash 0) \/ ([r = Crashed] /\ crashed)}}.
+Proof.
+  induction n; simpl; intros.
+
+  eapply Conseq.
+  apply CHalt.
+  apply pimpl_refl.
+  simpl.
+  pred.
+  
+  eapply Conseq.
+  econstructor.
+  eauto.
+  simpl.
+  intros.
+  eapply Conseq.
+  apply IHn.
+  pred.
+  simpl.
+  intros.
+  apply pimpl_refl.
+  apply pimpl_refl.
+  pred.
+Qed.
+
+
+(** * A log-based transactions implementation *)
+
+Definition disjoint (r1 : addr * nat) (r2 : addr * nat) :=
+  forall a, fst r1 <= a < fst r1 + snd r1
+    -> ~(fst r2 <= a < fst r2 + snd r2).
+
+Fixpoint disjoints (rs : list (addr * nat)) :=
+  match rs with
+    | nil => True
+    | r1 :: rs => Forall (disjoint r1) rs /\ disjoints rs
+  end.
+
+Record xparams := {
+  DataStart : addr; (* The actual committed data start at this disk address. *)
+    DataLen : nat;  (* Size of data region *)
+
+  LogLength : addr; (* Store the length of the log here. *)
+
+   LogStart : addr; (* Start of log region on disk *)
+     LogLen : nat;  (* Size of log region *)
+
+       Temp : addr; (* Temporary slot for use by library code *)
+
+   Disjoint : disjoints ((DataStart, DataLen)
+     :: (LogLength, 1)
+     :: (LogStart, LogLen)
+     :: (Temp, 1)
+     :: nil)
+}.
+
+Theorem upd_eq : forall m a v a',
+  a' = a
+  -> upd m a v a' = v.
+Proof.
+  intros; subst; unfold upd.
+  destruct (eq_nat_dec a a); tauto.
+Qed.
+
+Theorem upd_ne : forall m a v a',
+  a' <> a
+  -> upd m a v a' = m a'.
+Proof.
+  intros; subst; unfold upd.
+  destruct (eq_nat_dec a' a); tauto.
+Qed.
+
+Ltac disjoint' xp :=
+  generalize (Disjoint xp); simpl; intuition;
+    repeat match goal with
+             | [ H : True |- _ ] => clear H
+             | [ H : Forall _ nil |- _ ] => clear H
+             | [ H : Forall _ (_ :: _) |- _ ] => inversion_clear H
+           end; unfold disjoint in *; simpl in *; subst.
+
+Ltac disjoint'' a :=
+  match goal with
+    | [ H : forall a', _ |- _ ] => specialize (H a); omega
+  end.
+
+Ltac disjoint xp :=
+  disjoint' xp;
+  match goal with
+    | [ _ : _ <= ?n |- _ ] => disjoint'' n
+  end.
+
+Hint Rewrite upd_eq upd_ne using (congruence
+  || match goal with
+       | [ xp : xparams |- _ ] => disjoint xp
+     end).
+
+Ltac corr :=
+  ((apply CHalt || apply CCrash || apply CRead || apply CWrite
+    || eapply CSeq)
+  || (eapply Conseq; [ | apply pimpl_refl | ])); intros.
+
+
+Module Type LOG.
+  (* Methods *)
+  Parameter begin : xparams -> prog.
+  Parameter commit : xparams -> prog.
+  Parameter read : xparams -> addr -> prog.
+  Parameter write : xparams -> addr -> valu -> prog.
+
+  (* Representation invariant *)
+  Parameter rep : xparams
+    -> mem (* Memory as modified by current transaction,
+            * only consulted for addresses in data range *)
+    -> pred.
+
+  (* Specs *)
+  Axiom begin_ok : forall xp m, {{diskIs m}} (begin xp)
+    {{r, ([r = Crashed] /\ diskIs m) \/ rep xp m}}.
+End LOG.
+
+Module Log : LOG.
+  Definition begin xp :=
+    (LogLength xp) <-- 0.
+
+  Definition commit xp :=
+    len <- !(LogLength xp);
+    Loop i < len
+      Invariant [True]
+      OnCrash [True] Begin
+      a <- !(LogStart xp + 2*i);
+      v <- !(LogStart xp + 2*i + 1);
+      a <-- v
+    Pool.
+
+  Definition read xp a :=
+    len <- !(LogLength xp);
+    (Temp xp) <-- len;;
+
+    Loop i < len
+      Invariant [True]
+      OnCrash [True] Begin
+      a' <- !(LogStart xp + 2*i);
+      if eq_nat_dec a' a then
+        tmp <- !(Temp xp);
+        if eq_nat_dec tmp len then
+          (Temp xp) <-- a
+        else
+          Halt
+      else
+        Halt
+     Pool;;
+
+     tmp <- !(Temp xp);
+     if eq_nat_dec tmp len then
+       !a
+     else
+       !(LogStart xp + 2*tmp + 1).
+
+  Definition write xp a v :=
+    len <- !(LogLength xp);
+    if le_lt_dec (LogLen xp) len then
+      Crash
+    else
+      (LogStart xp + 2*len) <-- a;;
+      (LogStart xp + 2*len + 1) <-- v;;
+      (LogLength xp) <-- (S len).
+
+  Definition rep xp (m : mem) := (
+    (* Quantify over log. *)
+    exists ls,
+      (* The right log length is stored. *)
+      (LogLength xp) |-> (length ls)
+
+      (* This log is stored in the real memory. *)
+      /\ (foral i a_v, [nth_error (ls : list (addr * valu)) i = Some a_v]
+        --> (LogStart xp + 2*i) |-> (fst a_v))
+      /\ (foral i a_v, [nth_error ls i = Some a_v]
+        --> (LogStart xp + 2*i + 1) |-> (snd a_v))
+
+      (* The final log entry for each address is in the abstract memory. *)
+      /\ [forall i a_v, nth_error ls i = Some a_v
+        -> (forall j a_v', j > i -> nth_error ls i = Some a_v'
+          -> fst a_v' <> fst a_v)
+        -> m (fst a_v) = snd a_v]
+
+      (* Unupdated addresses are unchanged. *)
+      /\ (foral a, [DataStart xp <= a < DataStart xp + DataLen xp]
+        --> [forall i a_v, nth_error ls i = Some a_v
+          -> fst a_v <> a]
+        --> a |-> m a)
+  )%pred.
+
+
+  Lemma rep_nil : forall xp m,
+    rep xp m (upd m (LogLength xp) 0).
+  Proof.
+    exists nil; pred;
+      try match goal with
+            | [ _ : nth_error nil ?X = Some _ |- _ ] =>
+              destruct X; discriminate
+          end.
+  Qed.
+
+  Hint Resolve rep_nil.
+
+  Theorem begin_ok : forall xp m, {{diskIs m}} (begin xp) {{r, ([r = Crashed] /\ diskIs m) \/ rep xp m}}.
+  Proof.
+    repeat (corr || pred).
+  Qed.
+End Log.
